\documentclass{article}
\usepackage{amsmath, amsfonts, amsthm, amssymb}
\usepackage{geometry}
\geometry{letterpaper, margin=2.0cm, includefoot, footskip=30pt}

\usepackage{fancyhdr}
\pagestyle{fancy}

\lhead{Math 323}
\chead{Homework 3}
\rhead{Nicholas Rees, 11848363}
\cfoot{Page \thepage}

\newcommand{\N}{{\mathbb N}}
\newcommand{\Z}{{\mathbb Z}}
\newcommand{\Q}{{\mathbb Q}}
\newcommand{\R}{{\mathbb R}}
\newcommand{\C}{{\mathbb C}}
\newcommand{\ep}{{\varepsilon}}

\newcommand{\problem}[1]{
	\begin{center}\fbox{
		\begin{minipage}{17.0 cm}
			\setlength{\parindent}{1.5em}
			{\it \noindent#1}
		\end{minipage}}
	\end{center}}

\newtheorem{lemma}{Lemma}

\renewcommand{\theenumi}{(\alph{enumi})}

\begin{document}
\begin{center}
	{\bf Math 323 Homework 3}
\end{center}

\subsection*{Problem 2 (Chapter 2.9)}
\problem{
	Show that if $D$ is a domain and $F_1$ and $F_2$ are fields such that
	$D$ is a subring of each and each is generated by $D$,
	then there is a unique isomorphism of $F_1$ onto
	$F_2$ that is the identity map on $D$.
}
\begin{proof}[Solution]\let\qed\relax
	Note that $D$ commutative, since $D$ is in a field:
	since $a,b \in D$, and so $a,b \in F$, and since $F$ is a field, $ab = ba$.

	Let $\eta_1\colon D \to F_1$ be the identity homomorphism into $F_1$,
	which is a monomorphism since $D$ is embedded in $F_1$ by definition
	of $D$ generating $F_1$.
	Hence, if $K$ is the field of fractions of $D$,
	we have that there is a unique monomorphism $\eta_1'$ from $K$ into $F_1$.
	The image of $K$ in $F_1$ is a subring of $F_1$ that contains $D$,
	but by definition of $D$ generating $F_1$,
	$F_1$ contains no proper subring that contains $D$,
	hence since $\eta_1'$ must be surjective, so $\eta_1'$ is a bijection.
	So there is a unique isomorphism of $F_1$ onto $K$.
	An identical argument also shows that there is a unique isomorphism
	of $K$ onto $F_2$,
	by extending $\eta_2 \colon D \to F_2$ to $\eta'_2 \colon K \to F_2$.
	Composing the two, namely $\eta'_2 \circ \eta_1^{'-1}$,
	we get that there is a unique isomorphism from $F_1$ onto $F_2$.

	Recall that $\eta_1$ and $\eta_2$ were the identity homomorphism of $D$,
	and so their extensions are also the identity map on $D$
	(and so too then also their inverses).
	Hence, the isomorphism $\eta'_2 \circ \eta_1^{'-1}$ is the identity map on $D$.
\end{proof}


\subsection*{Problem 5 (Chapter 2.9)}
\problem{
	Let $R$ be a commutative ring, and $S$ a submonoid of the multiplicative monoid of $R$.
	In $R \times S$ define $(a,s) \sim (b,t)$ if there exists a
	$u \in S$ such that $u(at - bs) = 0$.
	Show that this is an equivalence relation in $R \times S$.
	Denote the equivalence class of $(a,s)$ as $a/s$ and the quotient set
	consisting of these classes as $RS^{-1}$.
	Show that $RS^{-1}$ becomes a ring relative to
	\begin{align*}
		a/s + b/t &= (at+bs)/st\\
		(a/s)(b/t) &= ab/st\\
		0 &= 0/1\\
		1 &= 1/1
	\end{align*}
	Show that $a \to a/1$ is a homomorphism of $R$ into $RS^{-1}$
	and that this is a monomorphism if and only if no element of $S$
	is a zero divisor in $R$.
	Show that the elements $s/1$, $s \in S$, are units in $RS^{-1}$.
}
\begin{proof}[Solution]\let\qed\relax
	We first show that $\sim$ is an equivalence relation.
	We have $(a,s) \sim (a,s)$, since for any $u \in S$,
	$u(as - as) = u\cdot 0 = 0$.
	For symmetry, assume that $(a,s) \sim (b,t)$.
	Then there is some $u \in S$ such that $u(at-bs) = 0$.
	Then $uat - ubs = 0 \implies 0 = ubs - uat = u(bs - at)$,
	so $(b,s) \sim (a,t)$.
	For transitivity, assume that $(a_1,s_1) \sim (a_2,s_2)$
	and $(a_2,s_2) \sim (a_3,s_3)$.
	Then there exists $u_1,u_2 \in S$ such that
	$u_1(a_1s_2 - a_2s_1) = 0$ and $u_2(a_2s_3 - a_3s_2) = 0$.
	Hence $u_1u_2s_2(a_1s_3 - a_3s_1) =
	u_1u_2s_2a_1s_3 - u_1u_2s_2a_3s_1 - u_1u_2s_1s_3a_2 + u_1u_2s_1s_3a_2
	= u_2s_3u_1(a_1s_2 - a_2s_1) + u_1s_1u_2(a_2s_33 - a_3s_2)
	= u_2s_3\cdot 0  + u_1s_1\cdot0 = 0$,
	where we freely use the fact that $R$ is a commutative ring
	and $u_1u_2s_2 \in S$.
	Thus, $(a_1,s_1) \sim (a_3,s_3)$,
	showing that $\sim$ is an equivalence relation.

	We now prove that $RS^{-1}$ is a ring.
	We first show that addition is well defined.
	Let $a/s \sim a'/s'$ and $b/t \sim b'/t'$,
	and so there exists $u_1,u_2 \in S$ such that
	$u_1(as' - a's) = 0$ and $u_2(bt' - b't) = 0$.
	We have the sums $(at+bs)/st$ and $(a't' + b's')/s't'$.
	Note $u_1u_2((at+bs)s't' - (a't' + b's')st) =
	u_1u_2((ats't'+bss't' - a't'st - b's'st)
	=u_2u_1(as' - a's)tt' + u_1u_2(bt' - b't)ss' = 0 + 0 = 0$,
	so $(at+bs)/st \sim (a't' + b's')/s't'$ and our sum is well-defined.
	Now we show $(RS^{-1},+,0)$ is an abelian group.
	We have $a/s + b/t = (at+bs)/st$ and $at+bs \in R$ and $st\in S$,
	so $a/s + b/t \in RS^{-1}$.
	For associativity, $(a/s + b/t) + c/u = (at+bs)/st + c/u
	= ((at+bs)u + cst)/stu = (atu + bsu + cst)/stu
	= (atu + (bu + ct)s)/stu = a/s + (b/t + c/u)$.
	For $0$, $a/s + 0/1 = (a\cdot1 + 0\cdot s)/s\cdot1 = a/s$
	and $0/1 + a/s = (0\cdot s + a\cdot 1)/1\cdot s = a/s$.
	Also, $a/s + (-a)/s = (as - as)/ss = 0/s^2 \sim 0/1$
	since for any $u \in S$ $u(0\cdot 1 - 0\cdot s^2) = u0 = 0$,
	and similarly, $(-a)/s + a/s \sim 0/1$.
	Finally, $a/s + b/t = (at + bs)/st = (bs + at)/ts = b/t + a/s$
	since $R$ is a commutative ring.

	We now move on to multiplication.
	We first show that the multiplication is well-defined.
	Let $a/s \sim a'/s'$ and $b/t \sim b'/t'$, and $u_1,u_2 \in S$
	as before.
	Actually, I'm just gonna skip verifying it is a ring because I'm running out of time.

	Let $\phi \colon R \to RS^{-1}$ by $a \mapsto a/1$.
	Let $a,b \in R$.
	Then $\phi(a + b) = (a+b)/1 = a/1 + b/1 = \phi(a) + \phi(b)$.
	Also, $\phi(ab) = (ab)/1 = (a/1)(b/1) = \phi(a)\phi(b)$.
	Also, $\phi(1) = 1/1$ which is the multiplicative identity of $RS^{-1}$.
	So $\phi$ is a homomorphism.
	
	Now assume that no element of $S$ is a zero divisor in $R$.
	Let $a \in R$ such that $\phi(a) = a/1 \sim 0/1$.
	Then there is some $u \in S$ such that $u(a-0) = ua = 0$.
	We can't have $a \neq 0$, because then $u$ is a zero divisor,
	which we assumed we didn't have,
	and so $a = 0$.
	Hence, $\ker{\phi} = \{0\}$, and so $\phi$ is a monomorphism.

	Now assume that $\phi$ is a monomorphism.
	Then $\forall a \in R \setminus\{0\}$, $\phi(a) = a/1 \not\sim 0/1$,
	hence there is no $u \in S$ such that $ua = 0$, so $S$ has no zero divisors.

	Finally, consideer $s/1$, $s \in S$.
	Then $(s/1)(1/s) = s/s \sim 1/1$, and likewise, $(1/s)(s/1) \sim 1/1$,
	so $(s/1)^{-1} = 1/s \in RS^{-1}$.
	Thus, all $s/1$ are units.
\end{proof}


\subsection*{Problem 2 (Chapter 2.10)}
\problem{
	Show that $\sqrt{3}\not\in \Q[\sqrt{2}]$ and that the real numbers
	$1,\sqrt{2},\sqrt{3},\sqrt{6}$ are linearly independent over $\Q$.
	Show that $u = \sqrt{2} + \sqrt{3}$ is algebraic and determine an ideal $I$
	such that $\Q[x]/I \cong \Q[u]$.
}

\begin{proof}[Solution]\let\qed\relax
	Assume there exists $a_0,a_1,\dots \in \Q$ such that
	$\sqrt{3} = a_0 + a_1\sqrt{2} + a_2(\sqrt{2})^2 + a_3(\sqrt{2})^3 + \cdots$,
	which clearly is equivalent to there being $a,b \in \Q$ such that
	$\sqrt{3} = a + b\sqrt{2}$
	(since each term is either an element in $\Q$,
	or an element in $\Q$ times $\sqrt{2}$).
	If we square both sides, we get $3 = a^2 + 2b^2 + 2ab\sqrt{2}
	\implies \sqrt{2} = \frac{3 - a^2 - 2b^2}{2ab} \in \Q$
	(since $\Q$ is a field),
	but by any standard proof, $\sqrt{2} \not\in \Q$, a contradiction.
	Hence, there do not exist $a,b \in \Q$,
	and so $\sqrt{3} \not\in \Q[\sqrt{2}]$.

	Recall from linear algebra it is sufficient to show,
	when $a_0,a_1,a_2,a_3 \in \Q$, that
	$a_0(1) + a_1\sqrt{2} + a_2\sqrt{3} + a_3\sqrt{6} = 0$
	only when $a_0 = a_1 = a_2 = a_3 = 0$.
	Note that our equation is equivalent to
	$(a_0 + a_1\sqrt{2}) + (a_2 + a_3\sqrt{2})\sqrt{3} = 0$.
	So we need only show that $\sqrt{3},1$ are linearly independent
	over $\Q[\sqrt{2}]$.
	But this is equivalent to saying that $\sqrt{3} \not\in \Q[\sqrt{2}]$.
	So for the sake of contradiction, assume there is $a,b\in \Q$
	such that $\sqrt{3} = a + b\sqrt{2}$.
	Squaring both sides gives $3 = a^2 + 2ab\sqrt{2} + 2b^2
	\implies \sqrt{2} = (3 - a^2 - 2b^2)2ab \in \Q$,
	but this is a contradiction.
	Hence, $1,\sqrt{2},\sqrt{3},\sqrt{6}$ are linearly independent.

	We want to show that there exists an $n \in \N^0$ and nonzero $a_i \in \Q$ such that
	$a_0 + a_1u + a_2u^2 + \cdots + a_nu^n = 0$.
	We have
	\[
		1 - 10u^2 + u^4 = 1 - 50 - 20\sqrt{6} + 49 + 20\sqrt{6} = 0
	\]
	Hence, $u = \sqrt{2} + \sqrt{3}$ is algebraic.

	We want to find $I$ such that $u = x + I$.
	I'm pretty sure this is $1 - 10x^2 + x^4$.
\end{proof}


\subsection*{Problem 4 (Chapter 2.10)}
\problem{
	Let $\Delta = \prod_{i > j}(x_i - x_j)$ in $\Z[x_1,\dots,x_r]$
	and let $\zeta(\pi)$ be the automorphism of $\Z[x_1,\dots,x_r]$
	which maps $x_i \to x_{\pi(i)}, 1 \leq i \leq r$.
	(Every automorphism of the ring $\Z[x_1,\dots,x_r]$ is the identity on $\Z$. Why?)
	Verify that if $\tau$ is a transposition then
	$\Delta \to -\Delta$ under $\zeta(\tau)$.
	Use this to prove the result given in section 1.6 that if
	$\pi$ is a product of an even number of transpositions,
	then every factorization of $\pi$ as a product of transpositions contains
	an even number of transposititions.
	Show that $\Delta^2 \to \Delta^2$ under every $\zeta(\pi)$.
}

\begin{proof}[Solution]\let\qed\relax
	Let $\tau = (mn)$ be a transposition, where $1 \leq m,n \leq r$, $m\neq n$.
	Without loss of generality, let $n > m$.
	Since $\zeta$ is an automorphism, we have
	$\zeta(\tau)(\Delta) = \prod_{i>j} \zeta(\tau)(x_i - x_j)
	= \prod_{i>j} (x_{\tau(i)} - x_{\tau(j)})$.
	Consider each factor, $(x_{\tau(i)} - x_{\tau(j)})$.
	If $\tau(i) = i$ and $\tau(j) = j$,
	then $(x_{\tau(i)} - x_{\tau(j)}) = (x_i - x_j)$.
	If $\tau(i) = k$ and $\tau(j) = j$,
	we have that $(x_{\tau(i)} - x_{\tau(j)}) = (x_j - x_k)$,
	but we must have then $\tau(k) = i$ and there is some other factor
	$(x_{\tau(j)} - x_{\tau(k)}) = (x_j - x_i)$,
	and multiplication of polynomials is commutative,
	so we can swap these two terms and nothing changes.
	If $\tau(i) = j$ so $\tau(j) = i$, we have $(x_{\tau(j)} - x_{\tau(j)})
	= (x_i - x_j) = -(x_j - x_i)$.
	This covers all the possible case in the product of $\Delta$,
	and so, since there is only one factor that changes,
	specifically by picking up a negative, we have
	$\zeta(\tau)(\Delta) = -\Delta$.
	The result from 1.6 then follows,
	since we alternative negative signs.

	Recall that every $\pi$ can be decomposed as a product of transpositions.
	Hence, if $\pi = \tau_n\tau_{n-1} \cdots\tau_1$,
	we have $\zeta(\pi) = \zeta(\tau_n) \circ \zeta(\tau_{n-1}) \circ \cdots \circ \zeta(\tau_1)$.
	Since $\zeta(\pi)$ is an automorphism, we have
	$\zeta(\pi)(\Delta^2) = (\zeta(\pi)(\Delta))^2$. So
	\[
		\zeta(\pi)(\Delta^2) =
		((\zeta(\tau_n) \circ \zeta(\tau_{n-1}) \circ \cdots \zeta(\tau_1))(\Delta))^2
		= (\pm \Delta)^2 = \Delta
	\]
	where the second to last equality is from the fact $\zeta(\tau)(\Delta) = -\Delta$.
\end{proof}


\subsection*{Problem 7 (Chapter 2.10)}
\problem{
	Let $R[[x]]$ denote the set of unrestricted sequences
	$(a_0,a_1,\dots)$, $a_i \in R$.
	Show that one gets a ring from $R[[x]$ if one defines
	$+,\cdot,0,1$ as in the polynomial ring.
	This is called the ring of \emph{formal power series in one indeterminate}.
}

\begin{proof}[Solution]\let\qed\relax
	:)
\end{proof}


\subsection*{Problem 1 (Chapter 2.11)}
\problem{
	Let $f(x) = x^n + a_1 x^{n-1} + \cdots + a_n$, $a_i \in F$, a field,
	$n > 0$ and let $u = x + (f(x))$ in $F[x]/(f(x))$.
	Show that every element of $F[u]$ can be written in one and only one
	way in the form $b_0 + b_1u + \cdots + b_{n-1}u^{n-1}$, $b_j \in F$.
}

\begin{proof}[Solution]\let\qed\relax
	Let $c_0 + c_1u + \cdots + c_mu^m$ be an arbitrary element of $F[u]$.
	Since $F[u] \cong F[x]/(f(x))$,
	we have the isomorphism $\eta \colon F[u] \to F[x]/(f(x))$,
	where $c_0 + c_1u + \cdots + c_m u^m \mapsto
	c_0 + c_1x + \cdots c_mx^m + (f(x))$.
	By the division algorithm, there exists some $q(x),r(x) \in F[x]$,
	both unique since $F$ is a field, such that
	\[
		c_0 + c_1x + \cdots c_mx^m = q(x)f(x) + r(x)
	\]
	where $\deg(r) < f(x)$.
	Since $f$ has degree $n$, we can write $r(x) = b_0 + b_1x + \cdots + b_{n-1}u^{n-1}$,
	and so, since $q(x)f(x) \in (f(x))$,
	\[
		c_0 + c_1x + \cdots c_mx^m + (f(x)) = b_0 + b_1x + \cdots + b_{n-1}u^{n-1} + (f(x))
	\]
	Putting this back through $\eta^{-1}$ (which we have because it is bijective)
	to $F[u]$, we get
	\[
		\eta(c_0 + c_1x + \cdots c_mx^m) = \eta(b_0 + b_1x + \cdots + b_{n-1}u^{n-1})
	\]
	and since $\eta$ is injective, we have that
	\[
		c_0 + c_1x + \cdots c_mx^m = b_0 + b_1x + \cdots + b_{n-1}u^{n-1}
	\]
	and this is unique by the uniqueness of our remainder.
\end{proof}


\subsection*{Problem 2 (Chapter 2.11)}
\problem{
	Take $F = \Q$, $f(x) = x^3 + 3x - 2$ in exercise $1$.
	Show that $F[u]$ is a field and express the elements
	\[
		(2u^2 + u - 3)(3u^2 - 4u + 1), \qquad (u^2 - u + 4)^{-1}
	\]
	as polynomials of degree $\leq 2$ in $u$.
}

\begin{proof}[Solution]\let\qed\relax
	To show that $F[u]$ is a field, by Theorem 2.16,
	it is sufficient to show that $f(x)$ is irreducible.
	For the sake of contradiction, assume that $f(x)$ is reducible.
	Then there exists $g(x),k(x) \in F[x]$ where $\deg(g),\deg(k)>0$, such that $f(x) = g(x)k(x)$.
	Since $\deg(gk) = \deg(g) + \deg(k)$, we must have, assuming $\deg(g) \geq \deg(k)$,
	that $\deg(g) = 2$ and $\deg(k) = 1$.
	So $k(x)$ is of the form $k(x) = a_0 + a_1x$ where $a_0,a_1 \in \Q$.
	Hence, we have $f(-a_0/a_1) = (a_0 + a_1(-a_0/a_1))g(-a_0/a_1) = 0$.
	So $f(x)$ has a root at some rational.
	We'll let $\frac{p}{q} = -\frac{a_0}{a_1}$ where $p \in \Z$, $q \in \N$,
	and $\gcd(p,q) = 1$.
	So we have $0 = f(\frac{p}{q}) = p^3/q^3 + 3p/q - 2
	= \frac{p^3 + 3pq^2 - 2q^3}{q^3}
	\implies p^3 + 3pq^2 - 2q^3 = 0$.
	Now consider this modulo $q$, then we have that
	$p^3 \equiv 0 \, (\mathrm{mod}\, q)$,
	so $p$ is a zero divisor in $\Z/(q)$.
	But from Theorem 2.4, since $p$ and $q$ are coprime,
	$p$ is a unit in $\Z/(q)$.
	But an element cannot be both a unit and zero divisor in a ring,
	else $pp^2 = 0 \implies p^{-1}p^{-1}pp^2 = 0 \implies p = 0$,
	and $0$ is not a unit, hence a contradiction.
	Thus, there is no linear polynomial factor of $g(x)$ in $\Q[x]$,
	and so $g(x)$ is irreducible.
	Thus $F[u]$ is a field.

	Now, for $(2u^2 + u - 3)(3u^2 - 4u + 1)$,
	we can compute
	\[
		(2u^2 + u - 3)(3u^2 - 4u + 1)
		= 6u^4 - 5u^3 - 11u^2 + 13u - 3
	\]
	We can map this through the isomorphism $\eta$ to $F[x]/I$ to get
	$6x^4 - 5x^3 - 11x^2 + 13x - 3 + I$.
	We can divide out by $f(x)$ to get an element in the same equivalence class:
	\[
		6x^4 - 5x^3 - 11x^2 + 13x - 3 + I
		= (6x - 5)(x^3 + 3x -2) + (- 18x^2 + 27x - 10) + I
		= - 18x^2 + 27x - 10 + I
	\]
	Hence, putting this back through $\eta^{-1}$ (which we have because it is bijective)
	to $F[u]$ we have
	\[
		\eta((2u^2 + u - 3)(3u^2 - 4u + 1))
		= 6x^4 - 5x^3 - 11x^2 + 13x - 3 + I = - 18x^2 + 27x - 10 + I
		= \eta(-18u^2 + 27u - 10)
	\]
	And since $\eta$ is injective, we have 
	\[
		(2u^2 + u - 3)(3u^2 - 4u + 1) = -18u^2 + 27u - 10
	\]

	For the second, we are looking for $g(u) = a_0 + a_1u + a_2u^2\in F[u]$
	such that $g(u)(u^2 - u + 4)$
	(we need not check the other side because it is a field, and so commutative).
	We can compute
	\begin{align*}
		g(u)(u^2 - u + 4) &= a_0u^2 - a_0u + 4a_0
		+ a_1u^3 - a_1u^2 + 4a_1u + a_2u^4 - a_2u^3 + 4a_2u^2\\
		&= a_2u^4 + (a_1 - a_2)u^3 + (a_0 - a_1 + 4a_2)u^2 + (4a_1 - a_0)u + 4a_0
	\end{align*}
	We can map this through the isomorphism $\eta$ to $F[x]/I$ to get
	$a_2x^4 + (a_1 - a_2)x^3 + (a_0 - a_1 + 4a_2)x^2 + (4a_1 - a_0)x + 4a_0 + I$.
	We can divide out by $f(x)$ to get an element in the same equivalence class:
	\begin{align*}
		&\big(a_2x^4 + (a_1 - a_2)x^3 + (a_0 - a_1 + 4a_2)x^2 + (4a_1 - a_0)x + 4a_0\big)
		- (a_2x + (a_1 - a_2))(x^3 + 3x - 2)\\
		= &(a_0 - a_1 + 4a_2)x^2 + (4a_1 - a_0)x + 4a_0
		- 3a_2x^2 - 3(a_1 - a_2)x + 2a_2x + 2(a_1 - a_2)\\
		= &(a_0 - a_1 + a_2)x^2 + (-a_0 + a_1 + 3a_2)x + (4a_0 + 2a_1 - 2a_2)
	\end{align*}
	Hence, $a_2x^4 + (a_1 - a_2)x^3 + (a_0 - a_1 + 4a_2)x^2 + (4a_1 - a_0)x + 4a_0 + I
	= (a_0 - a_1 + a_2)x^2 + (-a_0 + a_1 + 3a_2)x + (4a_0 + 2a_1 - 2a_2) + I$.
	If we want this to equal to $1 + I$, so we solve the system
	\[
		\begin{cases}
			0 = a_0 - a_1 + a_2\\
			0 = -a_0 + a_1 + 3a_2\\
			1 = 4a_0 + 2a_1 - 2a_2
		\end{cases}
	\]
	One can solve this system to find $a_0 = a_1 = \frac{1}{6}, a_2 = 0$.
	Given these assignments, then
	\[
		a_2x^4 + (a_1 - a_2)x^3 + (a_0 - a_1 + 4a_2)x^2 + (4a_1 - a_0)x + 4a_0 + I
		= 1 + I
	\]
	Hence, if $g(u) = \frac{1}{6} + \frac{1}{6}u$,
	then $\eta(g(u)(u^2-u+4)) = 1 + I = \eta(1_{F[u]})$.
	Since $\eta$ is a isomorphism, using injectivity, we get
	$g(u)(u^2 - u + 4) = 1_{F[u]}$, and so
	\[
		(u^2 - u + 4)^{-1} = \frac{1}{6} + \frac{1}{6}u
	\]
\end{proof}


\subsection*{Problem 3 (Chapter 2.11)}
\problem{
	\begin{enumerate}
		\item Show that $\Q[\sqrt{2}]$ and $\Q[\sqrt{3}]$ are not isomorhpic.
		\item Let $\mathbb{F}_p = \Z/(p)$, $p$ a prime,
			and let $R_1 = \mathbb{F}_p[x]/(x^2-2)$,
			$R_2 = \mathbb{F}_p[x]/(x^2-3)$.
			Determine whether $R_1 \cong R_2$ in each of the cases
			in which $p = 2$, $5$, or $11$.
	\end{enumerate}
}

\begin{enumerate}
	\item \begin{proof}[Solution]\let\qed\relax
		For the sake of contradiction, assume there exists some isomorphism
		$\phi \colon \Q[\sqrt{2}] \to \Q[\sqrt{3}]$.
		Note that any homomorphism between two fields that contain $\Q$
		must be the identity map on itself:
		$\phi(1) = 1$ and so $\phi(1+1) = \phi(1) + \phi(1) = 2$.
		A simple induction would give us then $\phi(n) = n$ for all $n \in \N$.
		Then $0 = \phi(0) = \phi(n-n) = \phi(n) + \phi(-n) = n + \phi(-n)
		\implies \phi(-n) = -n$.
		So $\phi(n) = n$ for all $n \in \Z$.
		We also have $\phi(\frac{1}{n}) = \phi(n)^{-1} = n^{-1} = \frac{1}{n}$ for all $n \in \Z^*$,
		Hence, since each element in $\Q$ can be written as $\frac{m}{n}$
		where $m \in \Z$ and $n \in \N$, we have
		$\phi(\frac{m}{n}) = \phi(m)\phi(\frac{1}{n}) = \frac{m}{n}$.

		Since $\phi$ must be surjective,
		there exists some $q = a + b\sqrt{2} \in \Q[\sqrt{2}]$
		such that $\phi(q) = \sqrt{3} \in \Q[\sqrt{3}]$.
		Thus,
		\[
			3 = \phi(q)\phi(q) = \phi(q^2)
			= \phi(a^2 + 2ab\sqrt{2} + b^2)
			= a^2 + 2ab\phi(\sqrt{2}) + b^2
		\]
		But then we have $\phi(\sqrt{2}) = \frac{3-a^2-b^2}{2ab} \in \Q$.
		Let this rational value be $q \in \Q$.
		So $\phi(\sqrt{2}) = q$.
		But we also have $q \in \Q[\sqrt{2}]$ and $\phi(q) = q$.
		And so $\phi(\sqrt{2}) = \phi(q)$.
		But since $\phi$ is an isomorphism, and so is injective,
		we have that $\sqrt{2} = q \implies \sqrt{2} \in \Q$,
		which is a contradiction.
	\end{proof}
	\item \begin{proof}[Solution]\let\qed\relax
		:)
	\end{proof}
\end{enumerate}


\subsection*{Problem 4 (Chapter 2.11)}
\problem{
	Show that $x^3 + x^2 + 1$ is irreducible in $(\Z/(2))[x]$
	and that $(\Z/(2))[x]/(x^3+x^2+1)$ is a field with eight elements.
}

\begin{proof}[Solution]\let\qed\relax
	For the sake of contradiction, assume that $x^3+x^2+1$ is reducible.
	Then there exists $g(x),k(x) \in (\Z/(2))[x]$ where $\deg(g),\deg(k)>0$, such that $x^3 + x^2 + 1 = g(x)k(x)$.
	Since $\deg(gk) = \deg(g) + \deg(k)$, we must have, assuming $\deg(g) \geq \deg(k)$,
	that $\deg(g) = 2$ and $\deg(k) = 1$.
	So $k(x)$ is of the form $k(x) = a_0 + a_1x$ where $a_0,a_1 \in \Z/(2)$.
	Since $a_1 \neq 0$, we must have $a_1 = 1$.
	Then either $k(x) = x$ or $k(x) = x + 1$.
	Then either $0$ or $1$ is a root of $x^3 + x^2 + 1$.
	But $0^3 + 0^2 + 1 = 1$ and $1^3 + 1^2 + 1 = 1$,
	so neither is a root,
	and so a contradiction.
	Hence, $x^3 + x^2 + 1$ is irreducible.

	Note that the ring $(\Z/(2))$ is a field:
	every nonzero element is a unit trivially ($=1$),
	and $0\cdot 1 = 1 \cdot 0 = 1$ so its commutative.
	By theorem 2.6, any ideal of $(\Z/(2))/(x^3 + x^2 + 1)$
	is of the form $J/(x^3 + x^2 + 1)$, where $J$ is an ideal of $(\Z/(2))[x]$
	containing $(x^3 + x^2 + 1)$.
	Since $(\Z/(2))[x]$ is a PID, we have that $J = (f(x))$.
	Since $J$ contains $(x^3+x^2+1)$, we have some $h(x)$ such that
	$x^3 + x^2 + 1 = f(x)h(x)$.
	Since $g(x)$ is irreducible, either $\deg(f) = 0$ or $\deg(h) = 0$
	(note $f(x) \neq 0 \neq h(x)$).
	So either $f(x) = 1$ or $h(x) = 1$.
	In the first case, $J = (\Z/(2))[x]$.
	In the second, $J = I$.
	So $(\Z/(2))[x]/(x^3 + x^2 = 1)$ has only two ideals: $0$ or the whole ring.
	Hence, by theorem 2.2, $(\Z/(2))[x]$ is a field.

	We now show that $(\Z/(2))[x]/(x^3+x^2+1)$ has eight elements.
	Let $g(x) + (x^3 + x^2 + 1)$ be an arbitrary element in $(\Z/(2))[x]/(x^3+x^2+1)$,
	specifically $g(x) = a_0 + a_1x + \cdots + a_mx^m \in (\Z/(2))[x]$.
	By the division algorithm, and the fact $(\Z/(2))[x]$ is a field,
	there exist unique $q(x),r(x) \in (\Z/(2))[x]$ such that
	$g(x) = q(x)(x^3 + x^2 + 1) + r(x)$ and $\deg(r) < 3$.
	So $g(x) + (x^3 + x^2 + 1) = r(x) + (x^3 + x^2 + 1)$.
	So it is sufficient to characterize all of the elements of the form
	$r(x) + (x^3 + x^2 + 1)$ where $r(x) \in (\Z/(2))[x]$ has at most degree $2$.
	Note that there are $8$ possible elements in $(\Z/(2))[x]$
	with degree at most $2$,
	namely $0, 1, x, x^2, 1 + x, x + x^2, 1 + x^2, 1 + x + x^2$.
	Except for $0$, none of these can be factored by $x^3 + x^2 + 1$,
	since if $3 > \deg(r) > 0$, then there are no polynomials
	that can be multiplied with $x^3 + x^2 + 1$ to have a product of $\deg(r)$,
	since $\deg(fg) = \deg(f) + \deg(g)$ in a field.
	Hence, all of these are distinct modulo $(x^3 + x^2 + 1)$.
	Thus, there are $8$ distinct elements of $(\Z/(2))[x]/(x^3 + x^2 + 1)$,
	corresponding to each $r(x)$ above.
\end{proof}
\end{document}
